Make request response example compatible with development branch

src/request_response/DY.Example.RequestResponse.Protocol.Stateful.Proof.fst
@@ -4,6 +4,8 @@ open Comparse
 open DY.Core
 open DY.Lib
 
+open CustomTactics
+
 open DY.Example.RequestResponse.Protocol.Total
 open DY.Example.RequestResponse.Protocol.Total.Proof
 open DY.Example.RequestResponse.Protocol.Stateful
@@ -12,38 +14,45 @@ open DY.Example.RequestResponse.Protocol.Stateful
 
 (*** State Predicates ***)
 
-#push-options "--ifuel 3 --z3rlimit 50"
+#push-options "--ifuel 2 --z3rlimit 100"
 let state_predicates_protocol: local_state_predicate protocol_state = {
   pred = (fun tr prin sess_id st ->
     match st with
     | ClientSendRequest {server; cmeta_data; nonce} -> (
       let client = prin in
-      comm_meta_data_knowable tr message_t client cmeta_data /\
+      comm_client_state_invariant tr message_t client cmeta_data /\
       is_secret (comm_label client server) tr nonce
     )
     | ServerReceiveRequest {client; nonce} -> (
       let server = prin in
-      is_knowable_by (comm_label client server) tr nonce
+      is_secret (comm_label client server) tr nonce \/
+        is_well_formed message_t (is_publishable tr) (Request {client; nonce})
     )
     | ClientReceiveResponse {server; cmeta_data; nonce} -> (
       let client = prin in
-      comm_meta_data_knowable tr message_t client cmeta_data /\
+      comm_client_state_invariant tr message_t client cmeta_data /\
       is_secret (comm_label client server) tr nonce
     )
   );
   pred_later = (fun tr1 tr2 prin sess_id st -> ());
-  pred_knowable = (fun tr prin sess_id st -> (
+  pred_knowable = (fun tr prin sess_id st -> 
+    let lab = principal_typed_state_content_label prin (DY.Lib.State.Typed.tag #protocol_state) sess_id st in
     match st with
     | ClientSendRequest {server; cmeta_data; nonce} -> (
+      assert(is_knowable_by lab tr nonce);
       comm_meta_data_knowable_proof tr message_t protocol_state sess_id st prin cmeta_data;
       ()
     )
-    | ServerReceiveRequest {client; nonce} -> ()
+    | ServerReceiveRequest {client; nonce} -> (
+      assert(is_knowable_by lab tr nonce);
+      ()
+    )
     | ClientReceiveResponse {server; cmeta_data; nonce} -> (
+      assert(is_knowable_by lab tr nonce);
       comm_meta_data_knowable_proof tr message_t protocol_state sess_id st prin cmeta_data;
       ()
     )
-  ));
+  );
 }
 #pop-options
 
@@ -55,6 +64,19 @@ let all_sessions = [
   private_keys_tag_and_invariant;
   state_predicate_and_tag_communication_layer_reqres message_t;
   mk_local_state_tag_and_pred state_predicates_protocol;
+]
+
+let state_update_predicate_protocol: local_state_update_predicate #crypto_invariants_protocol protocol_state = {
+  update_pred = (fun tr prin sess_id b1 b2 -> True);
+  update_pred_later = (fun tr1 tr2 prin sess_id b1 b2 -> ());
+  update_pred_trans = (fun tr prin sess_id b1 b2 b3 -> ());
+}
+
+let all_state_update_preds = [
+  pki_tag_and_state_update_pred;
+  private_keys_tag_and_state_update_pred;
+  state_update_predicates_communication_layer_and_tag message_t;
+  mk_local_state_tag_and_update_pred state_update_predicate_protocol;
 ]
 
 (*** Event Predicates ***)
@@ -82,6 +104,7 @@ let all_events = event_predicate_communication_layer_reqres_and_tag comm_layer_e
 
 let trace_invariants_protocol: trace_invariants = {
   state_pred = mk_state_pred all_sessions;
+  state_update_pred = mk_state_update_pred all_state_update_preds;
   event_pred = mk_event_pred all_events;
 }
 
@@ -100,14 +123,20 @@ let _ = (
   do_split_boilerplate mk_state_pred_correct all_sessions
 )
 let _ = (
+  assert_norm(List.Tot.no_repeats_p (List.Tot.map fst_dtuple (all_state_update_preds)));
+  do_split_boilerplate mk_state_update_pred_correct all_state_update_preds
+)
+let _ = (
   assert_norm(List.Tot.no_repeats_p (List.Tot.map fst (all_events)));
   do_split_boilerplate mk_event_pred_correct all_events
 )
+
+let _:squash (has_communication_layer_reqres_predicates comm_layer_event_preds) = ()
 #pop-options
 
 (*** Proofs ***)
 
-#push-options "--ifuel 3 --fuel 1"
+#push-options "--ifuel 0 --fuel 0 --z3rlimit 100"
 val client_send_request_proof:
   tr:trace ->
   comm_keys_ids:communication_keys_sess_ids ->
@@ -122,11 +151,26 @@ val client_send_request_proof:
   ))
   [SMTPat (trace_invariant tr); SMTPat (client_send_request comm_keys_ids client server tr)]
 let client_send_request_proof tr comm_keys_ids client server =
-  enable_reqres_comm_layer_lemmas comm_layer_event_preds;
-  ()
+  let (nonce, tr_nc) = mk_rand NoUsage (comm_label client server) 32 tr in
+  assert(trace_invariant tr_nc);
+  let payload = Request {client; nonce} in
+  let (x_snd, tr_snd) = send_request comm_keys_ids client server payload tr_nc in
+  
+  send_request_proof tr_nc comm_keys_ids comm_layer_event_preds client server payload;
+  assert(trace_invariant tr_snd);
+  match x_snd with
+  | None -> ()
+  | Some (msg_id, cmeta_data) -> (
+    let (sid, tr_sid) = new_session_id client tr_snd in
+    assert(trace_invariant tr_sid);
+    let (x_st, tr_st) = set_state client sid (ClientSendRequest { server; cmeta_data; nonce } <: protocol_state) tr_sid in
+    derive_comm_client_state_invariant tr_sid comm_layer_event_preds client cmeta_data;
+    assert(trace_invariant tr_st);
+    ()
+  )
 #pop-options
 
-#push-options "--ifuel 3 --fuel 1 --z3rlimit 50"
+#push-options "--ifuel 0 --fuel 0 --z3rlimit 50"
 val server_receive_request_send_response_proof:
   tr:trace ->
   comm_keys_ids:communication_keys_sess_ids ->
@@ -142,15 +186,95 @@ val server_receive_request_send_response_proof:
   ))
   [SMTPat (trace_invariant tr); SMTPat (server_receive_request_send_response comm_keys_ids server msg_id tr)]
 let server_receive_request_send_response_proof tr comm_keys_ids server msg_id =
-  enable_reqres_comm_layer_lemmas comm_layer_event_preds;
-  ()
+  let (_, tr_out) = server_receive_request_send_response comm_keys_ids server msg_id tr in
+  let (x_recv, tr_recv) = receive_request comm_keys_ids server msg_id tr in
+  receive_request_proof tr comm_keys_ids comm_layer_event_preds server msg_id;
+  assert(trace_invariant tr_recv);
+  match x_recv with
+  | None -> assert(tr_recv == tr_out)
+  | Some (msg, req_meta_data) -> (
+    let (x_gd, tr_gd) = guard_tr (Request? msg) tr_recv in
+    assert(trace_invariant tr_gd);
+    match x_gd with
+    | None -> assert(tr_gd == tr_out)
+    | Some () -> (
+      let Request req = msg in
+      let (sid, tr_sid) = new_session_id server tr_gd in
+      assert(trace_invariant tr_sid);
+      let ((), tr_st) = set_state server sid (ServerReceiveRequest { client=req.client; nonce=req.nonce } <: protocol_state) tr_sid in
+      assert(trace_invariant tr_st) by (
+        let open FStar.Tactics in
+        let _ = tcut (quote (squash (
+          let ((), tr_st) = set_state #protocol_state #local_state_protocol_state server sid (ServerReceiveRequest { client=req.client; nonce=req.nonce } <: protocol_state) tr_sid in
+          trace_invariant tr_st
+        ))) in
+
+        smt ();
+
+        apply_lemma (`set_state_invariant);
+        exact (`state_predicates_protocol);
+        exact (`state_update_predicate_protocol);
+        let _ = repeatn 4 split in
+
+        norm [delta_only [`%Mklocal_state_predicate?.pred; `%state_predicates_protocol]; iota];
+        let _ = pose_lemma (quote request_message_properties_send_request tr_sid comm_layer_event_preds req_meta_data) in
+        let _ = repeatn 3 smt in
+        assumption' ();
+        let _ = repeatn 2 smt in
+
+        dump "";
+        //admit_all ();
+        ()
+      );
+      let (x_snd, tr_snd) = send_response server req_meta_data (Response req.nonce) tr_st in
+      assert(trace_invariant tr_snd) by (
+        let open FStar.Tactics in
+        let _ = tcut (quote (squash (
+            let (_, tr_snd) = send_response server req_meta_data (Response req.nonce) tr_st in
+            trace_invariant tr_snd
+        ))) in
+
+        smt ();
+
+        apply_lemma (`send_response_proof);
+        exact (`comm_layer_event_preds);
+
+        let _ = repeatn 4 split in
+        assumption' ();
+        smt ();
+        smt ();
+
+        norm [delta_only [`%Mkcomm_reqres_higher_layer_event_preds?.send_response; `%comm_layer_event_preds; `%default_comm_reqres_higher_layer_event_preds]; iota];
+        exact (`());
+
+let c = tcc (cur_env ()) (quote request_message_properties_request' tr_st comm_layer_event_preds req_meta_data) in
+dump (comp_to_string c);
+  let pre, post =
+    match c with
+    | C_Lemma pre post _ -> pre, post
+    | C_Total res -> print (term_to_ast_string res); fail "a"
+    | _ -> fail ""
+  in
+        let _ = pose_lemma (quote request_message_properties_request' tr_st comm_layer_event_preds req_meta_data) in
+        let _ = repeatn 2 smt in
+
+        //dump "";
+        //admit_all ();
+        ()
+      );
+      assert(tr_snd == tr_out);
+      ()
+    )
+  )
 #pop-options
 
-#push-options "--ifuel 4 --fuel 1 --z3rlimit 40"
+
+#push-options "--ifuel 0 --fuel 0 --z3rlimit 30"
 val client_receive_response_proof:
   tr:trace ->
   client:principal ->
-  sid:state_id -> msg_id:timestamp ->
+  sid:state_id ->
+  msg_id:timestamp ->
   Lemma
   (requires
     trace_invariant tr
@@ -161,6 +285,65 @@ val client_receive_response_proof:
   ))
   [SMTPat (trace_invariant tr); SMTPat (client_receive_response client sid msg_id tr)]
 let client_receive_response_proof tr client sid msg_id =
-  enable_reqres_comm_layer_lemmas comm_layer_event_preds;
-  ()
+  let (_, tr_out) = client_receive_response client sid msg_id tr in
+
+  let (x_st, tr_st) = get_state client sid tr in
+  assert(trace_invariant tr_st);
+  match x_st with
+  | None -> assert(tr_st == tr_out)
+  | Some cstate ->
+    let (x_gd1, tr_gd1) = guard_tr (ClientSendRequest? cstate) tr_st in
+    assert(trace_invariant tr_gd1);
+    match x_gd1 with
+    | None -> assert(tr_gd1 == tr_out)
+    | Some () ->
+      let ClientSendRequest { server; cmeta_data; nonce } = cstate in
+
+      let (x_recv, tr_recv) = receive_response client cmeta_data msg_id tr_gd1 in
+      receive_response_proof tr_gd1 comm_layer_event_preds client cmeta_data msg_id;
+      assert(trace_invariant tr_recv);
+      match x_recv with
+      | None -> assert(tr_recv == tr_out)
+      | Some (msg, _) ->
+        let (x_gd2, tr_gd2) = guard_tr (Response? msg) tr_recv in
+        assert(trace_invariant tr_gd2);
+        match x_gd2 with
+        | None -> assert(tr_gd2 == tr_out)
+        | Some () ->
+          let Response res = msg in
+          let (x_gd3, tr_gd3) = guard_tr (res = nonce) tr_gd2 in
+          assert(trace_invariant tr_gd3);
+          match x_gd3 with
+          | None -> assert(tr_gd3 == tr_out)
+          | Some () ->
+            let ((), tr_set) = set_state client sid (ClientReceiveResponse { server; cmeta_data; nonce } <: protocol_state) tr_gd3 in
+            assert(trace_invariant tr_set) by (
+              let open FStar.Tactics in
+              let _ = tcut (quote (squash (
+                let ((), tr_set) = set_state #protocol_state #local_state_protocol_state client sid (ClientReceiveResponse { server; cmeta_data; nonce } <: protocol_state) tr_gd3 in
+                trace_invariant tr_set
+              ))) in
+
+              smt ();
+
+              apply_lemma (`set_state_invariant);
+              exact (`state_predicates_protocol);
+              exact (`state_update_predicate_protocol);
+              let _ = repeatn 4 split in
+
+              norm [ delta_only [`%Mklocal_state_predicate?.pred; `%state_predicates_protocol]; iota];
+
+              split ();
+              apply_lemma (quote derive_comm_client_state_invariant tr_gd3 comm_layer_event_preds client);
+              let _ = repeatn 3 smt in
+              assumption' ();
+              let _ = repeatn 2 smt in 
+
+              dump "";
+              //admit_all ();
+              ()
+            );
+            
+            assert(tr_set == tr_out);
+            ()
 #pop-options
