src/CustomTactics.fst
@@ -1,0 +1,47 @@
+module CustomTactics
+
+open FStar.Tactics
+
+#push-options "--ifuel 1"
+private
+let rec __assumption_aux' (bs : list binding) : Tac unit =
+    match bs with
+    | [] ->
+        fail "no assumption matches goal"
+    | b::bs ->
+        let t = binder_to_term b in
+        let typ = tc (cur_env()) t in
+        try (
+          t_exact false false t
+        ) with | _ ->
+        try (
+          apply (`FStar.Squash.return_squash);
+          if tmatch typ (cur_goal ()) then
+          t_exact false false t
+          else fail ""
+        ) with | _ ->
+        __assumption_aux' bs
+#pop-options
+
+let assumption' () : Tac unit =
+    __assumption_aux' (cur_vars ())
+
+let grewrite' = grewrite
+
+(*let grewrite' (t1 t2 : term) : Tac unit =
+    let e = tcut (mk_sq_eq t1 t2) in
+    let e = pack_ln (Tv_Var (bv_of_binder e)) in
+    pointwise (fun () ->
+      (* If the LHS is a uvar, do nothing, so we do not instantiate it. *)
+      let is_uvar =
+        match term_as_formula (cur_goal()) with
+        | Comp (Eq _) lhs rhs ->
+          (match inspect_ln lhs with
+           | Tv_Uvar _ _ -> true
+           | _ -> false)
+        | _ -> false
+      in
+      if is_uvar
+      then trefl ()
+      else try t_exact false false e with | _ -> trefl ())
+*)
